Sequence theory is now 1-based. Fixed unsoundness in loop writes. Optimized global invariant in the bg theory. OOM verifies.

eve/Src/Delivery/studio/tools/autoproof/base_theory.bpl
@@ -84,16 +84,6 @@ const unique owns: Field (Set ref); // Ghost field for owns set of an object.
 const unique observers: Field (Set ref); // Ghost field for observers set of an object.
 const unique subjects: Field (Set ref); // Ghost field for subjects set of an object.
 
-// Is o free? (owner is open)
-function {:inline} is_free(h: HeapType, o: ref): bool {
-	h[o, owner] == Void
-}
-
-// Is o wrapped in h? (closed and free)
-function {:inline} is_wrapped(h: HeapType, o: ref): bool {
-	h[o, closed] && is_free(h, o)
-}
-
 // Is o open in h? (not closed and free)
 function {:inline} is_open(h: HeapType, o: ref): bool {
 	!h[o, closed]
@@ -104,11 +94,20 @@ function {:inline} is_closed(h: HeapType, o: ref): bool {
 	h[o, closed]
 }
 
+// Is o free? (owner is open)
+function {:inline} is_free(h: HeapType, o: ref): bool {
+  h[o, owner] == Void
+}
+
+// Is o wrapped in h? (closed and free)
+function {:inline} is_wrapped(h: HeapType, o: ref): bool {
+	h[o, closed] && is_free(h, o)
+}
+
 // Only allocated references can be in ghost sets
 axiom (forall h: HeapType, o: ref, r: ref, f: Field (Set ref) :: h[o, allocated] && h[o, f][r] ==> h[r, allocated]);
-//axiom (forall h: HeapType, o: ref, r: ref :: h[o, observers][r] ==> h[r, allocated]);
-//axiom (forall h: HeapType, o: ref, r: ref :: h[o, owns][r] ==> h[r, allocated]);
-//axiom (forall h: HeapType, o: ref, r: ref :: h[o, subjects][r] ==> h[r, allocated]);
+// Only allocated references can be in ghost sequences
+axiom (forall h: HeapType, o: ref, r: ref, f: Field (Seq ref) :: h[o, allocated] && Seq#Contains(h[o, f], r) ==> h[r, allocated]);
 
 // Is o' in the ownership domain of o? Yes if they are equal, or both closed and o' is transitively owned by o
 function in_domain(h: HeapType, o: ref, o': ref): bool
@@ -148,29 +147,13 @@ function {:inline true} writable_domains(h: HeapType): bool
 }
 
 // Objects outside of ownership domains of mods did not change, unless they were newly allocated
-// function writes(h: HeapType, h': HeapType, mods: Set ref): bool { 
-	// (forall <T> o: ref, f: Field T :: { h[o, f] } { h'[o, f] }
-		// ((forall o': ref :: { mods[o'] } { in_domain(h, o', o) } mods[o'] ==> !in_domain(h, o', o)) &&
-		 // h[o, allocated])
-			// ==>
-		// h'[o, f] == h[o, f])
-	// &&
-	// no_garbage(h, h')
-// }
 function writes(h: HeapType, h': HeapType, mods: Frame): bool { 
 	(forall <T> o: ref, f: Field T :: { h[o, f] } { h'[o, f] }
     h[o, allocated] ==>      
       h'[o, f] == h[o, f] ||
       mods[o, f] ||
       (exists o': ref :: {mods[o', closed]}{in_domain(h, o', o)} o' != o && mods[o', closed] && in_domain(h, o', o))
-  ) &&
-	no_garbage(h, h')
-}
-
-// The allocation status of objects does not change
-function no_garbage(old_heap: HeapType, new_heap: HeapType): bool {
-	(forall o: ref :: { new_heap[o, allocated] } { old_heap[o, allocated] }
-		old_heap[o, allocated] ==> new_heap[o, allocated])
+  )
 }
 
 // ----------------------------------------------------------------------
@@ -180,7 +163,7 @@ function no_garbage(old_heap: HeapType, new_heap: HeapType): bool {
 function user_inv(h: HeapType, o: ref): bool;
 
 // Is object o closed or the invariant satisfied?
-function inv(h: HeapType, o: ref): bool {
+function {:inline true} inv(h: HeapType, o: ref): bool {
 	h[o, closed] ==> user_inv(h, o)
 }
 
@@ -190,11 +173,10 @@ function inv(h: HeapType, o: ref): bool {
 // Global heap invariants
 function {:inline true} global(h: HeapType): bool
 {
-	is_open(h, Void) && // G1
-	(forall o: ref :: h[o, allocated] && is_free(h, o) ==> (h[o, owner] == Void)) && // G2
-	(forall o: ref :: h[o, allocated] && is_open(h, o) ==> is_free(h, o)) && // G3
-	(forall o: ref, o': ref :: h[o, allocated] && h[o', allocated] && h[o, closed] && h[o, owns][o'] ==> (h[o', closed] && h[o', owner] == o)) && // G4
-	(forall o: ref :: h[o, allocated] && h[o, closed] ==> inv(h, o)) // G5
+  is_open(h, Void) &&
+  (forall o: ref :: h[o, allocated] && is_open(h, o) ==> is_free(h, o)) &&
+  (forall o: ref, o': ref :: {h[o, owns][o']} h[o, allocated] && h[o', allocated] && h[o, closed] && h[o, owns][o'] ==> (h[o', closed] && h[o', owner] == o)) && // G2
+  (forall o: ref :: {user_inv(h, o)}{h[o, allocated]} h[o, allocated] ==> inv(h, o)) // G1
 }
 
 // Allocate fresh object
@@ -216,6 +198,7 @@ procedure allocate(t: Type) returns (result: ref);
 
 // Update Heap position Current.field with value.
 procedure update_heap<T>(Current: ref, field: Field T, value: T);
+  requires (Current != Void) && (Heap[Current, allocated]);
 	requires field != closed && field != owner; // update tag:closed_or_owner_not_allowed UP4
 	requires is_open(Heap, Current); // update tag:target_open UP1
 	requires (forall o: ref :: Heap[Current, observers][o] ==> (is_open(Heap, o) || (user_inv(Heap, o) ==> user_inv(Heap[Current, field := value], o)))); // update tag:observers_open_or_inv_preserved UP2
@@ -227,6 +210,7 @@ procedure update_heap<T>(Current: ref, field: Field T, value: T);
 
 // Unwrap o
 procedure unwrap(o: ref);
+  requires (o != Void) && (Heap[o, allocated]); // pre tag:attached
 	requires is_wrapped(Heap, o); // pre tag:wrapped UW1
   requires writable[o, closed]; // pre tag:writable UW2
   modifies Heap;
@@ -238,6 +222,7 @@ procedure unwrap(o: ref);
   free ensures HeapSucc(old(Heap), Heap);
 
 procedure unwrap_all (Current: ref, s: Set ref);
+  requires (forall o: ref :: s[o] ==> (o != Void) && (Heap[o, allocated])); // pre tag:attached
 	requires (forall o: ref :: s[o] ==> is_wrapped(Heap, o)); // pre tag:wrapped UW1
   requires (forall o: ref :: s[o] ==> writable[o, closed]); // pre tag:writable UW2
   modifies Heap;
@@ -250,6 +235,7 @@ procedure unwrap_all (Current: ref, s: Set ref);
 
 // Wrap o
 procedure wrap(o: ref);
+  requires (o != Void) && (Heap[o, allocated]); // pre tag:attached
 	requires is_open(Heap, o); // pre tag:open W1
 	requires user_inv(Heap, o); // pre tag:invariant_holds W2
 	requires (forall o': ref :: Heap[o, owns][o'] ==> is_wrapped(Heap, o')); // pre tag:owned_objects_wrapped W3
@@ -263,6 +249,7 @@ procedure wrap(o: ref);
   free ensures HeapSucc(old(Heap), Heap);
 
 procedure wrap_all(Current: ref, s: Set ref);
+  requires (forall o: ref :: s[o] ==> (o != Void) && (Heap[o, allocated])); // pre tag:attached
 	requires (forall o: ref :: s[o] ==> is_open(Heap, o)); // pre tag:open W1
 	requires (forall o: ref :: s[o] ==> user_inv(Heap, o)); // pre tag:invariant_holds W2
 	requires (forall o: ref :: s[o] ==> (forall o': ref :: Heap[o, owns][o'] ==> is_wrapped(Heap, o'))); // pre tag:owned_objects_wrapped W3
