eve/Src/Delivery/studio/tools/autoproof/sequence.bpl
@@ -21,31 +21,34 @@ function Seq#Build<T>(s: Seq T, val: T): Seq T;
 axiom (forall<T> s: Seq T, v: T :: { Seq#Length(Seq#Build(s,v)) }
   Seq#Length(Seq#Build(s,v)) == 1 + Seq#Length(s));
 axiom (forall<T> s: Seq T, i: int, v: T :: { Seq#Index(Seq#Build(s,v), i) }
-  (i == Seq#Length(s) ==> Seq#Index(Seq#Build(s,v), i) == v) &&
-  (i != Seq#Length(s) ==> Seq#Index(Seq#Build(s,v), i) == Seq#Index(s, i)));
+  (i == Seq#Length(s) + 1 ==> Seq#Index(Seq#Build(s,v), i) == v) &&
+  (i <= Seq#Length(s) ==> Seq#Index(Seq#Build(s,v), i) == Seq#Index(s, i)));
 
 function Seq#Append<T>(Seq T, Seq T): Seq T;
 axiom (forall<T> s0: Seq T, s1: Seq T :: { Seq#Length(Seq#Append(s0,s1)) }
   Seq#Length(Seq#Append(s0,s1)) == Seq#Length(s0) + Seq#Length(s1));
 
 function Seq#Index<T>(Seq T, int): T;
-axiom (forall<T> t: T :: { Seq#Index(Seq#Singleton(t), 0) } Seq#Index(Seq#Singleton(t), 0) == t);
+axiom (forall<T> t: T :: { Seq#Index(Seq#Singleton(t), 1) } Seq#Index(Seq#Singleton(t), 1) == t);
 axiom (forall<T> s0: Seq T, s1: Seq T, n: int :: { Seq#Index(Seq#Append(s0,s1), n) }
-  (n < Seq#Length(s0) ==> Seq#Index(Seq#Append(s0,s1), n) == Seq#Index(s0, n)) &&
-  (Seq#Length(s0) <= n ==> Seq#Index(Seq#Append(s0,s1), n) == Seq#Index(s1, n - Seq#Length(s0))));
+  (n <= Seq#Length(s0) ==> Seq#Index(Seq#Append(s0,s1), n) == Seq#Index(s0, n)) &&
+  (Seq#Length(s0) < n ==> Seq#Index(Seq#Append(s0,s1), n) == Seq#Index(s1, n - Seq#Length(s0))));
 
 function Seq#Update<T>(Seq T, int, T): Seq T;
 axiom (forall<T> s: Seq T, i: int, v: T :: { Seq#Length(Seq#Update(s,i,v)) }
-  0 <= i && i < Seq#Length(s) ==> Seq#Length(Seq#Update(s,i,v)) == Seq#Length(s));
+  1 <= i && i <= Seq#Length(s) ==> Seq#Length(Seq#Update(s,i,v)) == Seq#Length(s));
 axiom (forall<T> s: Seq T, i: int, v: T, n: int :: { Seq#Index(Seq#Update(s,i,v),n) }
-  0 <= n && n < Seq#Length(s) ==>
+  1 <= n && n <= Seq#Length(s) ==>
     (i == n ==> Seq#Index(Seq#Update(s,i,v),n) == v) &&
     (i != n ==> Seq#Index(Seq#Update(s,i,v),n) == Seq#Index(s,n)));
 
-function Seq#Contains<T>(Seq T, T): bool;
+function Seq#Contains<T>(s: Seq T, x: T): bool;
 axiom (forall<T> s: Seq T, x: T :: { Seq#Contains(s,x) }
   Seq#Contains(s,x) <==>
-    (exists i: int :: { Seq#Index(s,i) } 0 <= i && i < Seq#Length(s) && Seq#Index(s,i) == x));
+    (exists i: int :: { Seq#Index(s,i) } 1 <= i && i <= Seq#Length(s) && Seq#Index(s,i) == x));
+axiom (forall<T> s: Seq T, i: int :: { Seq#Index(s,i) }
+  1 <= i && i <= Seq#Length(s) ==>
+    Seq#Contains(s, Seq#Index(s, i)));    
 axiom (forall x: ref ::
   { Seq#Contains(Seq#Empty(), x) }
   !Seq#Contains(Seq#Empty(), x));
@@ -62,19 +65,19 @@ axiom (forall<T> s: Seq T, n: int, x: T ::
   { Seq#Contains(Seq#Take(s, n), x) }
   Seq#Contains(Seq#Take(s, n), x) <==>
     (exists i: int :: { Seq#Index(s, i) }
-      0 <= i && i < n && i < Seq#Length(s) && Seq#Index(s, i) == x));
+      1 <= i && i <= n && i <= Seq#Length(s) && Seq#Index(s, i) == x));
 axiom (forall<T> s: Seq T, n: int, x: T ::
   { Seq#Contains(Seq#Drop(s, n), x) }
   Seq#Contains(Seq#Drop(s, n), x) <==>
     (exists i: int :: { Seq#Index(s, i) }
-      0 <= n && n <= i && i < Seq#Length(s) && Seq#Index(s, i) == x));
+      0 <= n && n + 1 <= i && i <= Seq#Length(s) && Seq#Index(s, i) == x));
 
 function Seq#Equal<T>(Seq T, Seq T): bool;
 axiom (forall<T> s0: Seq T, s1: Seq T :: { Seq#Equal(s0,s1) }
   Seq#Equal(s0,s1) <==>
     Seq#Length(s0) == Seq#Length(s1) &&
     (forall j: int :: { Seq#Index(s0,j) } { Seq#Index(s1,j) }
-        0 <= j && j < Seq#Length(s0) ==> Seq#Index(s0,j) == Seq#Index(s1,j)));
+        1 <= j && j <= Seq#Length(s0) ==> Seq#Index(s0,j) == Seq#Index(s1,j)));
 axiom (forall<T> a: Seq T, b: Seq T :: { Seq#Equal(a,b) }  // extensionality axiom for sequences
   Seq#Equal(a,b) ==> a == b);
 
@@ -82,7 +85,7 @@ function Seq#SameUntil<T>(Seq T, Seq T, int): bool;
 axiom (forall<T> s0: Seq T, s1: Seq T, n: int :: { Seq#SameUntil(s0,s1,n) }
   Seq#SameUntil(s0,s1,n) <==>
     (forall j: int :: { Seq#Index(s0,j) } { Seq#Index(s1,j) }
-        0 <= j && j < n ==> Seq#Index(s0,j) == Seq#Index(s1,j)));
+        1 <= j && j <= n ==> Seq#Index(s0,j) == Seq#Index(s1,j)));
 
 function Seq#Take<T>(s: Seq T, howMany: int): Seq T;
 axiom (forall<T> s: Seq T, n: int :: { Seq#Length(Seq#Take(s,n)) }
@@ -90,7 +93,7 @@ axiom (forall<T> s: Seq T, n: int :: { Seq#Length(Seq#Take(s,n)) }
     (n <= Seq#Length(s) ==> Seq#Length(Seq#Take(s,n)) == n) &&
     (Seq#Length(s) < n ==> Seq#Length(Seq#Take(s,n)) == Seq#Length(s)));
 axiom (forall<T> s: Seq T, n: int, j: int :: { Seq#Index(Seq#Take(s,n), j) } {:weight 25}
-  0 <= j && j < n && j < Seq#Length(s) ==>
+  1 <= j && j <= n && j <= Seq#Length(s) ==>
     Seq#Index(Seq#Take(s,n), j) == Seq#Index(s, j));
 
 function Seq#Drop<T>(s: Seq T, howMany: int): Seq T;
@@ -99,7 +102,7 @@ axiom (forall<T> s: Seq T, n: int :: { Seq#Length(Seq#Drop(s,n)) }
     (n <= Seq#Length(s) ==> Seq#Length(Seq#Drop(s,n)) == Seq#Length(s) - n) &&
     (Seq#Length(s) < n ==> Seq#Length(Seq#Drop(s,n)) == 0));
 axiom (forall<T> s: Seq T, n: int, j: int :: { Seq#Index(Seq#Drop(s,n), j) } {:weight 25}
-  0 <= n && 0 <= j && j < Seq#Length(s)-n ==>
+  0 <= n && 1 <= j && j <= Seq#Length(s)-n ==>
     Seq#Index(Seq#Drop(s,n), j) == Seq#Index(s, j+n));
 
 axiom (forall<T> s, t: Seq T ::
@@ -110,16 +113,16 @@ axiom (forall<T> s, t: Seq T ::
 // Commutability of Take and Drop with Update.
 axiom (forall<T> s: Seq T, i: int, v: T, n: int ::
   { Seq#Take(Seq#Update(s, i, v), n) }
-    0 <= i && i < n && n <= Seq#Length(s) ==> Seq#Take(Seq#Update(s, i, v), n) == Seq#Update(Seq#Take(s, n), i, v) );
+    1 <= i && i <= n && n <= Seq#Length(s) ==> Seq#Take(Seq#Update(s, i, v), n) == Seq#Update(Seq#Take(s, n), i, v) );
 axiom (forall<T> s: Seq T, i: int, v: T, n: int ::
   { Seq#Take(Seq#Update(s, i, v), n) }
-    n <= i && i < Seq#Length(s) ==> Seq#Take(Seq#Update(s, i, v), n) == Seq#Take(s, n));
+    n < i && i <= Seq#Length(s) ==> Seq#Take(Seq#Update(s, i, v), n) == Seq#Take(s, n));
 axiom (forall<T> s: Seq T, i: int, v: T, n: int ::
   { Seq#Drop(Seq#Update(s, i, v), n) }
-    0 <= n && n <= i && i < Seq#Length(s) ==> Seq#Drop(Seq#Update(s, i, v), n) == Seq#Update(Seq#Drop(s, n), i-n, v) );
+    0 <= n && n + 1 <= i && i <= Seq#Length(s) ==> Seq#Drop(Seq#Update(s, i, v), n) == Seq#Update(Seq#Drop(s, n), i-n, v) );
 axiom (forall<T> s: Seq T, i: int, v: T, n: int ::
   { Seq#Drop(Seq#Update(s, i, v), n) }
-    0 <= i && i < n && n < Seq#Length(s) ==> Seq#Drop(Seq#Update(s, i, v), n) == Seq#Drop(s, n));
+    1 <= i && i <= n && n < Seq#Length(s) ==> Seq#Drop(Seq#Update(s, i, v), n) == Seq#Drop(s, n));
 // drop commutes with build.
 axiom (forall<T> s: Seq T, v: T, n: int ::
   { Seq#Drop(Seq#Build(s, v), n) }
@@ -145,10 +148,11 @@ axiom Seq#Drop(Seq#Empty(), 0) == Seq#Empty();  // [][0..] == []
 // CUSTOM ADDITIONS
 
 // All reference elements in sequences are allocated
-axiom (forall h: HeapType, s: Seq ref, i: int :: 0 <= i && i <= Seq#Length(s) ==> h[Seq#Index(s, i), allocated]);
+// Replaced by a more sound one in base theory
+// axiom (forall h: HeapType, s: Seq ref, i: int :: 0 <= i && i <= Seq#Length(s) ==> h[Seq#Index(s, i), allocated]);
 
 // Conversion from sequence to set
-function Set#FromSeq<T>(Seq T): Set T;
-axiom (forall<T> q: Seq T, o: T :: { Set#FromSeq(q)[o] } Seq#Contains(q, o) <==> Set#FromSeq(q)[o]);
+function Seq#Range<T>(Seq T): Set T;
+axiom (forall<T> q: Seq T, o: T :: { Seq#Range(q)[o] }{ Seq#Contains(q, o) } Seq#Contains(q, o) <==> Seq#Range(q)[o]);
 
 
